löste det random ass problemet

Lab_4/Q2.dfy
@@ -1,12 +1,21 @@
 method ComputeFact(n : nat) returns (res : nat)
   requires n > 0
-  ensures res == fact(n);
+  ensures res == fact(n)
  {
   res := 1;
   var i := 2;
   while (i <= n) 
+  invariant (i <= n + 1) && (res == fact(i-1))
+  decreases n-i+1
   {
     res := res * i;
     i := i + 1;
   }
  }
+
+function fact(n: nat) : nat
+  requires n > 0
+  decreases n
+{
+  if n == 1 then 1 else n * fact(n-1)
+}
